src/dvspec/dafny/specification/dvn.dfy
@@ -69,13 +69,13 @@ module DV
                                     && signer in s.all_nodes
                                     && verify_bls_siganture(signing_root, att_share.signature, signer)
                         )
-                        && exists signers: set<BLSPubkey> ::
-                                && signers <= s.all_nodes
-                                && |signers| >= quorum(|s.all_nodes|)
-                                && forall signer: BLSPubkey ::
-                                        signer in signers
-                                            ==> exists att_share: AttestationShare ::
-                                                    verify_bls_siganture(signing_root, att_share.signature, signer)
+                        // && exists signers: set<BLSPubkey> ::
+                        //         && signers <= s.all_nodes
+                        //         && |signers| >= quorum(|s.all_nodes|)
+                        //         && forall signer: BLSPubkey ::
+                        //                 signer in signers
+                        //                     ==> exists att_share: AttestationShare ::
+                        //                             verify_bls_siganture(signing_root, att_share.signature, signer)
                                                     
 
                 )
@@ -94,13 +94,13 @@ module DV
                             && |verifiable_att_shares| >= quorum(|s.all_nodes|)
                             && (forall att_share |
                                     att_share in verifiable_att_shares :: att_share.data == data)
-                            && exists signers: set<BLSPubkey> ::
-                                && signers <= s.all_nodes
-                                && |signers| >= quorum(|s.all_nodes|)
-                                && forall signer: BLSPubkey ::
-                                        signer in signers
-                                            ==> exists att_share: AttestationShare ::
-                                                    verify_bls_siganture(signing_root, att_share.signature, signer)
+                            // && exists signers: set<BLSPubkey> ::
+                            //     && signers <= s.all_nodes
+                            //     && |signers| >= quorum(|s.all_nodes|)
+                            //     && forall signer: BLSPubkey ::
+                            //             signer in signers
+                            //                 ==> exists att_share: AttestationShare ::
+                            //                         verify_bls_siganture(signing_root, att_share.signature, signer)
 
                             ::
                                     && var signing_root := compute_attestation_signing_root(data, fork_version);
